\documentclass[]{report}
\usepackage{atlasphysics,amsmath}

\begin{document}

\section{Theoretical $\Zzero-\Zzero$ Cross Section $\sigma$}

Define

\begin{align*}
\alpha &= \frac{g^{4}}{(32\pi)^{2}s} \frac{\sqrt{1-4\varepsilon^{2}}}{(1-\lambda^{2})^{2} + (\frac{\lambda\Gamma_{\Zzero}}{\rts})},
\\
\beta &= ((C_{V}^{e})^{2} + (C_{A}^{e})^{2})((C_{V}^{\mu})^{2}),
\\
\Delta &= ((C_{V}^{e})^{2} + (C_{A}^{e})^{2})((C_{A}^{\mu})^{2}),
\\
\Gamma &= 8C_{V}^{e}C_{A}^{e}C_{V}^{\mu}C_{A}^{\mu}.
\end	{align*}

These definitions produce the differential cross section:

$$
\frac{\d\sigma}{\d\Omega}^{\Zzero-\Zzero}
  = \alpha(\beta(1+\cos^{2}{\theta}+4\varepsilon^{2}\sin^{2}{\theta})
    + \Delta(1+\cos^{2}{\theta})(1-4\varepsilon^{2})
    + \Gamma\sqrt{1-4\varepsilon^{2}}\cos{\theta}
  )
$$

Under the change of variable $\sin^{2}{\theta}\ra1-\cos^{2}{\theta}$ and the substitution

$$\varepsilon_{\pm}=1\pm4\varepsilon^{2},$$

we see that the integral over the solid angle $\d{\Omega} = \d{\phi}\d{(\cos{\theta})}$ becomes

\begin{align*}
\sigma &= 2\pi\alpha\int\limits_{-1}^{1}
  \beta\varepsilon_{+} + \beta\varepsilon_{-}x^{2} + \Delta\varepsilon_{-}
  + \Delta\varepsilon_{-}x^{2} + \Gamma\sqrt{\varepsilon_{-}}x
  \d{x}
  \\
  &= 2\pi\alpha\int\limits_{-1}^{1}
    \beta\varepsilon_{+} + \Delta\varepsilon_{-} + (\beta + \Delta)\varepsilon_{-}x^{2}
    + \Gamma\sqrt{\varepsilon_{-}}x
    \d{x}.
\end{align*}

The $\Gamma$ term will disappear as it is symmetric in the integration limits. After simplification, the trivial integral is evaluated to

$$
\sigma^{\Zzero-\Zzero} = 4\pi\alpha(\beta(\varepsilon_{+} + \frac{1}{3}\varepsilon_{-})
  + \frac{4}{3}\Delta\varepsilon_{-})
$$

\end{document}